F_mu_ref_conc/soundness_binary.v
@@ -16,28 +16,26 @@ Proof.
   eapply (wp_adequacy Σ); iIntros (?) "Hσ".
   iMod (auth_alloc to_heap ownP heapN _ ∅ with "[Hσ]")
     as (γh) "[#Hh1 Hh2]"; auto; first done.
-  iMod (own_alloc (● (to_cfg ([e'], ∅) : cfgUR)
-    ⋅ ◯ (({[ 0 := Excl' e' ]} : tpoolUR, ∅) : cfgUR))) as (γc) "[Hcfg1 Hcfg2]".
-  { rewrite -auth_both_op auth_valid_discrete /= prod_included /= to_empty_heap.
-    eauto using to_cfg_valid. }
-  iMod (inv_alloc specN _ (∃ ρ', own γc (● ρ') ★ (■ ([e'], ∅) →⋆ of_cfg ρ'))%I
-    with "[Hcfg1]") as "#Hcfg"; trivial.
-  { iNext. iExists _. iIntros "{$Hcfg1} !%". rewrite from_to_cfg; constructor. }
+  iMod (own_alloc (● (to_tpool [e'], ∅)
+    ⋅ ◯ (({[ 0 := Excl e' ]} : tpoolUR, ∅) : cfgUR))) as (γc) "[Hcfg1 Hcfg2]".
+  { apply auth_valid_discrete_2. split=>//. split=>//. apply to_tpool_valid. }
+  set (Hcfg := CFGSG _ (HeapIG _ _ _ γh) _ γc).
+  iMod (inv_alloc specN _ (spec_inv ([e'], ∅)) with "[Hcfg1]") as "#Hcfg".
+  { iNext. iExists [e'], ∅. rewrite {2}/to_heap fin_maps.map_fmap_empty. auto. }
   rewrite -(empty_env_subst e).
   iApply wp_fupd; iApply wp_wand_r; iSplitL; [iApply (bin_log_related_alt
-    (Hlog (CFGSG _ (HeapIG _ _ _ γh) _ γc)) [] [] ([e'], ∅) 0 [])|]; simpl.
+    (Hlog _) [] [] ([e'], ∅) 0 [])|]; simpl.
   { rewrite /heapI_ctx /spec_ctx /auth_ctx /tpool_mapsto /auth_own /=.
     rewrite empty_env_subst -interp_env_nil. by iFrame "Hh1 Hcfg Hcfg2". }
   iIntros (v1); iDestruct 1 as (v2) "[Hj #Hinterp]".
-  iInv specN as (ρ) ">[Hown Hsteps]" "Hclose"; iDestruct "Hsteps" as %Hsteps'.
+  iInv specN as (tp σ) ">[Hown Hsteps]" "Hclose"; iDestruct "Hsteps" as %Hsteps'.
   rewrite /tpool_mapsto /auth.auth_own /=.
-  iCombine "Hj" "Hown" as "Hown".
-  iDestruct (own_valid with "Hown") as %[[[tp h] Hρ] [Htp ?]]%auth_valid_discrete.
-  move: Hρ; rewrite /= right_id pair_op left_id leibniz_equiv_iff=> ?; simplify_eq/=.
-  iMod ("Hclose" with "[-]").
-  { iDestruct "Hown" as "[Ho1 Ho2]". rewrite /auth_inv; eauto. }
-  iIntros "!> !%". exists (of_tpool tp), (of_heap h), v2.
-  destruct tp as [|[[]|]]; by inversion_clear Htp.
+  iDestruct (own_valid_2 with "[$Hown $Hj]") as %Hvalid.
+  move: Hvalid=> /auth_valid_discrete_2
+    [/prod_included [/tpool_singleton_included Hv2 _] _].
+  destruct tp as [|? tp']; simplify_eq/=.
+  iMod ("Hclose" with "[-]") as "_"; [iExists (_ :: tp'), σ; auto|].
+  iIntros "!> !%"; eauto.
 Qed.
 
 Lemma binary_soundness Σ `{irisPreG lang Σ, authG Σ heapUR, authG Σ cfgUR}
